TODO some tinkering, moving to trestle-code?

Experiments/ProofChecking/RangeArray.lean
@@ -38,11 +38,11 @@ namespace RangeArray
 
 -- CC: TODO better names
 @[inline, always_inline]
-private def markIndexAsDeleted (i : Int) : Int :=
+def markIndexAsDeleted (i : Int) : Int :=
   if i ≥ 0 then -i - 1 else i
 
 @[inline, always_inline]
-private def getIndexFromMarkedIndex (i : Int) : Nat :=
+def getIndexFromMarkedIndex (i : Int) : Nat :=
   if i ≥ 0 then i.natAbs else i.natAbs - 1
 
 @[simp]
@@ -140,35 +140,6 @@ structure RangeArray (α : Type u) where
     RangeArray.getIndexFromMarkedIndex (Seq.get indexes ⟨i, lt_of_le_of_lt hij hj⟩) ≤
     RangeArray.getIndexFromMarkedIndex (Seq.get indexes ⟨j, hj⟩)
 
-/-
-CNF: <20 clauses>
-LRAT:
-
-21 1 4 -2 0 ...
-25 2 -10 0 ...
-
-data = [1, 5, 6, -2 | ]
-indexes = [0, -4, -4, -4, -4, ]
-indexes = [0, ]
-
-fold at an index (run a function across a single specified clause)
-folding across all indexes (hack this with Fin.foldRange [above])
-add a sub-array (adding a clause)
-delete (has something been deleted?)
-(Garbage collect)
-
-spec fns:
-- array α @ i (where i is not deleted)
-- array (array α) [all deleted clauses filtered out]
-
-proofs:
-- fold(M) at index i = fold(M) over (array @ i) or whatever
-- fold(M) = fold(M) over array
-- toArrays (delete RA) = RA' ↔ ∃ L M R, RA.toArrays = L ++ [M] ++ R ∧ RA'.toArrays = L ++ R
-- garbageCollect RA = RA' → RA.toArrays = RA'.toArrays
-
--/
-
 namespace RangeArray
 
 variable {α : Type u} (A : RangeArray α) (v : α)
@@ -205,6 +176,9 @@ def empty (size : Nat := 100) : RangeArray α := {
   h_indexes := by simp [LeanColls.size]
   h_indexes_inc := by simp [LeanColls.size]
 }
+
+instance instInhabited [Inhabited α] : Inhabited (RangeArray α) where
+  default := empty
 
 /-- Adds a single element to the underlying data array, without adding a new index. -/
 --@[inline, always_inline, specialize]
@@ -260,22 +234,6 @@ def index (i : Nat) : Nat :=
     indexFin A ⟨i, hi⟩
   else 0
 
-theorem indexFin_eq_index {A : RangeArray α} {i : Nat} (hi : i < A.size) : A.indexFin ⟨i, hi⟩ = A.index i := by
-  simp [index, hi]
-
-theorem indexFin_eq_index?' {A : RangeArray α} (i : Fin A.size) : A.indexFin i = A.index i.val := by
-  simp [index]
-
-theorem index_le_dataSize (i : Nat) : A.index i ≤ A.dsize := by
-  by_cases hi : i < A.size
-  <;> simp [index, hi]
-  exact A.h_indexes hi
-
-theorem index_le_index_of_le {i j : Nat} (hij : i ≤ j) (hj : j < A.size) :
-    A.index i ≤ A.index j := by
-  simp [index, hj, lt_of_le_of_lt hij hj]
-  exact A.h_indexes_inc hij hj
-
 /-- Checks whether the ith container is deleted. -/
 @[inline, always_inline]
 def isDeletedFin (i : Fin A.size) : Bool :=
@@ -286,13 +244,6 @@ def isDeletedFin (i : Fin A.size) : Bool :=
 def isDeleted (i : Nat) : Bool :=
   if hi : i < A.size then isDeletedFin A ⟨i, hi⟩
   else true
-
-theorem isDeletedFin_eq_isDeleted {A : RangeArray α} {i : Nat} (hi : i < A.size) :
-    A.isDeletedFin ⟨i, hi⟩ = A.isDeleted i := by
-  simp [isDeleted, hi]
-
-theorem isDeletedFin_eq_isDeleted' {A : RangeArray α} (i : Fin A.size) : A.isDeletedFin i = A.isDeleted i.val := by
-  simp [isDeleted]
 
 /-- Gets the size of the container under the provided index.
     The size of the most-recently-added container is the old `A.usize`.
@@ -312,24 +263,22 @@ def rsize (i : Nat) : Nat :=
   if hi : i < A.size then A.rsizeFin ⟨i, hi⟩
   else 0
 
-theorem rsizeFin_eq_rsize {A : RangeArray α} {i : Nat} (hi : i < A.size) : A.rsizeFin ⟨i, hi⟩ = A.rsize i := by
-  simp [rsize, hi]
-
-theorem rsizeFin_eq_rsize' {A : RangeArray α} (i : Fin A.size) : A.rsizeFin i = A.rsize i.val := by
-  simp [rsize]
-
-def deleteFin (i : Fin A.size) : RangeArray α := { A with
-  indexes := Seq.set A.indexes i (markIndexAsDeleted (Seq.get A.indexes i))
-  deletedSize := A.deletedSize + A.rsize i
+def deleteFin (i : Fin A.size) : RangeArray α :=
+  let dSize := A.deletedSize
+  let rSize := A.rsize i
+  let v := markIndexAsDeleted (Seq.get A.indexes i)
+  { A with
+  indexes := Seq.set A.indexes i v
+  deletedSize := dSize + rSize
   h_dataSize_empty := by simp; exact A.h_dataSize_empty
   h_indexes := by
-    simp [Seq.get_set]
+    simp [Seq.get_set, dSize, rSize, v]
     rcases i with ⟨i, hi⟩
     intro j hj
     by_cases hij : i = j
     <;> simp [hij, A.h_indexes]
   h_indexes_inc := by
-    simp [Seq.get_set]
+    simp [Seq.get_set, dSize, rSize, v]
     rcases i with ⟨i, hi⟩
     intro j k hjk hk
     by_cases hjk_eq : j = k
@@ -343,12 +292,6 @@ def deleteFin (i : Fin A.size) : RangeArray α := { A with
 
 def delete (i : Nat) : RangeArray α :=
   if hi : i < A.size then A.deleteFin ⟨i, hi⟩ else A
-
-theorem deleteFin_eq_delete {i : Nat} (hi : i < A.size) : A.deleteFin ⟨i, hi⟩ = A.delete i := by
-  simp [delete, hi]
-
-theorem deleteFin_eq_delete' (i : Fin A.size) : A.deleteFin i = A.delete i.val := by
-  simp [delete]
 
 -- CC: Can be implemented as `commit`, then `delete`.
 /-- Creates a new container that contains any elements added via `addElement`,
@@ -419,405 +362,6 @@ def append' (arr : Array α) := { A with
       exact A.h_indexes_inc hij _
 }
 
-section lemmas
-
-variable (A : RangeArray α) (v : α) (i : Nat)
-
-/-! # empty -/
-
-@[simp]
-theorem size_empty (n : Nat) : (empty n : RangeArray α).size = 0 := by
-  simp [size, empty, LeanColls.size]
-
-@[simp]
-theorem dsize_empty (n : Nat) : (empty n : RangeArray α).dsize = 0 := by
-  simp [empty, dsize]
-
-@[simp]
-theorem usize_empty (n : Nat) : (empty n : RangeArray α).usize = 0 := by
-  simp [empty, LeanColls.size, usize]
-
-/-! # push -/
-
-@[simp]
-theorem size_push : (A.push v).size = A.size := by simp [push, size]
-
-@[simp]
-theorem dsize_push : (A.push v).dsize = A.dsize := by simp [push, dsize]
-
-@[simp]
-theorem usize_push : (A.push v).usize = A.usize + 1 := by
-  simp [push, usize, dsize, Nat.sub_add_comm A.h_size]
-
-@[simp]
-theorem index_push : (A.push v).index i = A.index i := by
-  simp [push, index, indexFin]
-
-@[simp]
-theorem rsizeFin_push {A : RangeArray α} {i : Nat} (hi : i < A.size) (v : α) :
-    (A.push v).rsizeFin ⟨i, hi⟩ = A.rsizeFin ⟨i, hi⟩ := by
-  simp [rsizeFin]; rfl
-
-@[simp]
-theorem rsize_push : (A.push v).rsize i = A.rsize i := by
-  simp [rsize]
-
-@[simp]
-theorem isDeleted_push : (A.push v).isDeleted i = A.isDeleted i := by
-  simp [push, isDeleted, isDeletedFin, size]
-
-theorem delete_push_comm : (A.push v).delete i = (A.delete i).push v := by
-  simp [delete, deleteFin]
-  split
-  · congr 2
-  · rfl
-
-theorem clear_of_usize_zero : A.usize = 0 → A.clear = A := by
-  intro hu
-  simp [clear, hu]
-
-@[simp]
-theorem clear_push : (A.push v).clear = A.clear := by
-  simp [clear, push, Seq.snoc, Array.push, usize, dsize, LeanColls.size, Array.size_append]
-  have h_le := A.h_size
-  simp [dataSize, dsize, LeanColls.size] at h_le
-  unfold Array.size at h_le ⊢
-  split
-  · rename _ => h_eq
-    have : A.dataSize ≥ List.length A.data.data + 1 := Nat.le_of_sub_eq_zero h_eq
-    have := lt_of_succ_le this
-    exact absurd h_le (not_le.mpr this)
-  · rename _ => h_ne; clear h_ne
-    split
-    · rename _ => h_eq
-      congr
-      rw [← le_antisymm (Nat.le_of_sub_eq_zero h_eq) A.h_size]
-      conv => lhs; rw [← Nat.add_zero (List.length A.data.data)]
-      simp [List.take_append]
-    · have : List.take A.dataSize (A.data.data ++ [v]) = List.take A.dataSize A.data.data := by
-        rw [List.take_append_of_le_length h_le]
-      congr
-
-/-! # clear -/
-
-@[simp]
-theorem size_clear : A.clear.size = A.size := by
-  simp [clear, size]; split <;> rfl
-
-@[simp]
-theorem dsize_clear : A.clear.dsize = A.dsize := by
-  simp [clear, dsize]; split <;> rfl
-
-@[simp]
-theorem data_size_clear : Size.size (A.clear).data = A.dsize := by
-  simp [clear, dsize]
-  split <;> rename _ => h
-  · simp [usize, dsize] at h
-    exact le_antisymm (Nat.le_of_sub_eq_zero h) A.h_size
-  · simp [LeanColls.size]
-    exact A.h_size
-
-@[simp]
-theorem indexes_clear : A.clear.indexes = A.indexes := by
-  simp [clear, indexes]
-  split <;> rename _ => h
-  · rfl
-  · simp [LeanColls.size]
-
-@[simp]
-theorem usize_clear : A.clear.usize = 0 := by
-  simp [clear, usize]
-  split
-  · assumption
-  · simp [LeanColls.size]
-
-@[simp]
-theorem rsize_clear : A.clear.rsize i = A.rsize i := by
-  simp [clear, rsize]
-  split <;> rename _ => h
-  · split <;> rename _ => hi
-    · congr 2
-      simp [h]
-      exact size_clear A
-      aesop -- CC: ???
-    · rfl
-  · split <;> rename _ => hi
-    · -- Annoyingly, we must unpack rsizeFin to get rid of the `if`
-      -- We then put it back into rsizeFin for the data comparison
-      simp [rsizeFin_eq_rsize, h]
-      simp [rsize, hi, rsizeFin, size]
-      congr
-    · rfl
-
-@[simp]
-theorem clear_clear : A.clear.clear = A.clear := by
-  simp [clear, size, dsize, usize, LeanColls.size]
-  split <;> rename _ => h_usize
-  <;> simp [h_usize]
-
-
-/-! # delete -/
-
-@[simp]
-theorem size_delete : (A.delete i).size = A.size := by
-  rw [delete]; split <;> rename _ => hi <;> try rfl
-  simp [deleteFin, hi, size]
-
-@[simp]
-theorem size_deleteFin {A : RangeArray α} {i : Nat} (hi : i < A.size) :
-    (A.deleteFin ⟨i, hi⟩).size = A.size := by
-  simp [deleteFin, size]
-
-@[simp]
-theorem dsize_delete : (A.delete i).dsize = A.dsize := by
-  rw [delete]; split <;> rfl
-
-@[simp]
-theorem dsize_deleteFin {A : RangeArray α} {i : Nat} (hi : i < A.size) :
-    (A.deleteFin ⟨i, hi⟩).dsize = A.dsize := by
-  simp [deleteFin, dsize]
-
-@[simp]
-theorem usize_delete : (A.delete i).usize = A.usize := by
-  rw [delete]; split <;> rfl
-
-@[simp]
-theorem usize_deleteFin {A : RangeArray α} {i : Nat} (hi : i < A.size) :
-    (A.deleteFin ⟨i, hi⟩).usize = A.usize := by
-  simp [deleteFin, usize]
-
--- We cannot prove this theorem, because garbage collection will throw this off
---theorem index_delete_ne (A : RangeArray α) {i j : Nat} (hij : i ≠ j) :
---    (A.delete i).index j = A.index j := by
-
--- This theorem will hold, regardless of garbage collection
-theorem rsize_delete_ne {A : RangeArray α} {i j : Nat} (hij : i ≠ j) :
-    (A.delete i).rsize j = A.rsize j := by
-  simp [delete]
-  split <;> rename _ => hi <;> try rfl
-  simp [deleteFin, rsize, size]
-  split <;> rename _ => hj <;> try rfl
-  simp [rsizeFin, hi, hj, size, indexFin, Seq.get_set, hij]
-  split <;> rename _ => hj₂ <;> try rfl
-  split <;> rename _ => hi₂ <;> try rfl
-  simp [hi₂]
-
-@[simp]
-theorem isDeleted_delete_eq : (A.delete i).isDeleted i = true := by
-  by_cases hi : i < Size.size A.indexes
-  · simp [isDeleted, isDeletedFin, delete, deleteFin, hi,
-      Seq.get, Seq.set, RangeArray.markIndexAsDeleted]
-    split <;> omega
-  · simp [isDeleted, hi]
-
-theorem isDeleted_delete_ne (A : RangeArray α) {i j : Nat} (hij : i ≠ j) :
-    (A.delete i).isDeleted j = A.isDeleted j := by
-  simp [delete]
-  split <;> rename _ => hi <;> try rfl
-  simp [isDeleted]
-  split <;> rename _ => hj <;> try rfl
-  simp [isDeletedFin, deleteFin, hi, hj, size, indexFin, hij]
-
-theorem isDeleted_delete (i j : Nat) : (A.delete i).isDeleted j =
-    if i = j then true else A.isDeleted j := by
-  split <;> rename _ => hij
-  · subst hij; exact isDeleted_delete_eq A i
-  · exact isDeleted_delete_ne A hij
-
-theorem isDeleted_true_of_ge {A : RangeArray α} {i : Nat} (hi : i ≥ A.size) : A.isDeleted i = true := by
-  simp [isDeleted, hi]
-
-theorem lt_of_isDeleted_false {A : RangeArray α} {i : Nat} (hi : A.isDeleted i = false) : i < A.size := by
-  simp [isDeleted] at hi
-  split at hi
-  · assumption
-  · contradiction
-
-/-! # commit -/
-
-@[simp]
-theorem size_commit : A.commit.size = A.size + 1 := by
-  simp [commit, size]
-
-@[simp]
-theorem dsize_commit : A.commit.dsize = Size.size A.data := by
-  simp [commit, dsize]
-
-@[simp]
-theorem usize_commit : A.commit.usize = 0 := by
-  simp [usize, commit, dsize]
-
-theorem index_commit_lt {A : RangeArray α} {i : Nat} (hi : i < A.size) :
-    (A.commit).index i = A.index i := by
-  rw [size] at hi
-  simp [commit, size, hi, lt_succ_of_lt hi, index, indexFin, Seq.get_snoc]
-
-@[simp]
-theorem index_commit_eq : (A.commit).index A.size = A.dsize := by
-  simp [commit, index, indexFin, Seq.get_snoc, size]
-
-theorem index_commit_gt {A : RangeArray α} {i : Nat} (hi : i > A.size) :
-    (A.commit).index i = 0 := by
-  rw [size] at hi
-  simp [commit, index, indexFin, size, hi]
-  intro h
-  exact absurd hi (not_lt_of_ge (le_of_lt_succ h))
-
-@[simp]
-theorem rsize_commit_lt {A : RangeArray α} {i : Nat} (hi : i < A.size) :
-    (A.commit).rsize i = A.rsize i := by
-  rw [size] at hi
-  simp [commit, rsize, size, hi, lt_succ_of_lt hi, rsizeFin]
-  split <;> rename _ => hi'
-  · simp [indexFin, size, Seq.get_snoc, hi', lt_of_succ_lt hi']
-  · have := le_antisymm (Nat.succ_le_of_lt hi) (not_lt.mp hi')
-    rw [succ_eq_add_one] at this
-    simp [indexFin, size, this, Seq.get_snoc, getIndexFromMarkedIndex_coe, hi]
-
-@[simp]
-theorem rsizeFin_commit {A : RangeArray α} {i : Nat} (hi : i < A.size) :
-    (A.commit).rsizeFin ⟨i, by rw [size_commit]; exact Nat.lt_succ_of_lt hi⟩ = A.rsizeFin ⟨i, hi⟩ := by
-  simp [rsizeFin_eq_rsize]; exact rsize_commit_lt hi
-
-@[simp]
-theorem rsize_commit_eq : (A.commit).rsize A.size = A.usize := by
-  simp [commit, rsize, rsizeFin, dsize, size, index, indexFin, Seq.get_snoc]
-
-@[simp]
-theorem rsizeFin_commit_eq : (A.commit).rsizeFin ⟨A.size, by simp⟩ = A.usize := by
-  simp [rsizeFin_eq_rsize]
-
-@[simp]
-theorem rsize_commit_gt {A : RangeArray α} {i : Nat} (hi : i > A.size) :
-    (A.commit).rsize i = 0 := by
-  rw [size] at hi
-  simp [commit, rsize, rsizeFin, size, hi]
-  intro h
-  exact absurd hi (not_lt_of_ge (le_of_lt_succ h))
-
-@[simp]
-theorem clear_commit (A : RangeArray α) : A.commit.clear = A.commit := by
-  simp [commit, clear]
-
-theorem isDeleted_commit_lt {A : RangeArray α} {i : Nat} (hi : i < A.size) :
-    (A.commit).isDeleted i = A.isDeleted i := by
-  rw [size] at hi
-  simp [commit, isDeleted, isDeletedFin, size, hi, lt_succ_of_lt hi, Seq.get_snoc]
-
-@[simp]
-theorem isDeleted_commit_eq : (A.commit).isDeleted A.size = false := by
-  simp [commit, isDeleted, isDeletedFin, size, Seq.get_snoc]
-
-/-! # append -/
-
-@[simp]
-theorem append_empty (A : RangeArray α) : A.append Array.empty = A.clear.commit := by
-  simp [append, Array.empty, commit]
-
-@[simp]
-theorem append_empty' (A : RangeArray α) : A.append #[] = A.clear.commit := by
-  simp [append, Array.empty, commit]
-
-@[simp]
-theorem append_nil (A : RangeArray α) : A.append { data := [] } = A.clear.commit :=
-  append_empty A
-
-variable (arr : Array α)
-
-theorem append_eq_append'_aux :
-  ((arr.foldl (init := A) (fun A' v => A'.push v)) |>.commit) = A.append' arr := by
-  have ⟨L⟩ := arr
-  rw [append']
-  induction' L with x xs ih generalizing A
-  · simp [commit, LeanColls.size]
-  · rw [foldl_cons]
-    rw [ih (push A x)]
-    simp [push, Seq.snoc]
-    constructor
-    · have : A.data.push x = A.data ++ #[x] := rfl
-      rw [this]
-      rw [Array.append_assoc, Array.singleton_append_data_eq_cons]
-    · simp [LeanColls.size, succ_eq_add_one]
-      rw [add_assoc, add_comm 1 (List.length xs)]
-
-theorem append_eq_append' : A.append arr = (A.clear).append' arr := by
-  rw [append, append_eq_append'_aux A.clear arr]
-
-@[simp]
-theorem append_indexes : (A.append arr).indexes = Seq.snoc A.indexes (A.dsize : Int) := by
-  rw [append_eq_append']
-  simp [append']
-
-@[simp]
-theorem size_append : (A.append arr).size = A.size + 1 := by
-  have ⟨L⟩ := arr
-  cases L
-  · simp
-  · rw [append_eq_append']
-    simp [append', size]
-
-@[simp]
-theorem dsize_append : (A.append arr).dsize = A.dsize + Size.size arr := by
-  have ⟨L⟩ := arr
-  cases L
-  · simp [append, usize, dsize]; rfl
-  · simp [append_eq_append', append', dsize]
-
-theorem lt_size_append_of_lt_size {A : RangeArray α} {i : Nat} (hi : i < A.size)
-    (arr : Array α) : i < (A.append arr).size := by
-  simp; exact lt_succ_of_lt hi
-
-theorem index_append_lt {A : RangeArray α} {i : Nat} (hi : i < A.size) (arr : Array α) :
-    (A.append arr).index i = A.index i := by
-  rw [append_eq_append']
-  rw [size] at hi
-  simp [append', hi, lt_succ_of_lt hi, size]
-  simp [index, indexFin, size, hi, lt_succ_of_lt hi, Seq.get_snoc]
-
-@[simp]
-theorem index_append_eq : (A.append arr).index A.size = A.dsize := by
-  rw [append_eq_append', append']
-  simp [index, indexFin, size, Seq.get_snoc]
-
-theorem rsize_append_lt {A : RangeArray α} {i : Nat} (hi : i < A.size) (arr : Array α) :
-    (A.append arr).rsize i = A.rsize i := by
-  rw [append_eq_append']
-  rw [size] at hi
-  simp [append', hi, lt_succ_of_lt hi, size]
-  simp [rsize, rsizeFin, index, indexFin, size, hi, lt_succ_of_lt hi, Seq.get_snoc]
-  split <;> rename _ => hi'
-  · rfl
-  · have := le_antisymm (Nat.succ_le_of_lt hi) (not_lt.mp hi')
-    rw [succ_eq_add_one] at this
-    simp [this]
-
-@[simp]
-theorem rsize_append_eq : (A.append arr).rsize A.size = Size.size arr := by
-  rw [append_eq_append']
-  simp [rsize, size, append', rsizeFin, dsize]
-  rw [indexFin_eq_index]
-  simp
-  conv => lhs; lhs; rw [Nat.add_comm]
-  simp [index, indexFin, size]
-
-@[simp]
-theorem usize_append (arr : Array α) : (A.append arr).usize = 0 := by
-  simp [append_eq_append', append']
-
-theorem isDeleted_append_lt {A : RangeArray α} {i : Nat} (hi : i < A.size) (arr : Array α) :
-    (A.append arr).isDeleted i = A.isDeleted i := by
-  rw [append_eq_append']
-  rw [size] at hi
-  simp [append', hi, lt_succ_of_lt hi, size]
-  simp [isDeleted, isDeletedFin, hi, lt_succ_of_lt hi, Seq.get_snoc, size]
-
-@[simp]
-theorem isDeleted_append_eq : (A.append arr).isDeleted A.size = false := by
-  rw [append_eq_append']
-  simp [append', isDeleted, isDeletedFin, size, Seq.get_snoc]
-
-end lemmas
-
 /-! # get -/
 
 @[inline, always_inline]
@@ -830,69 +374,7 @@ def get [Inhabited α] (i : Nat) : α :=
     A.getFin ⟨i, hi⟩
   else default
 
-variable [Inhabited α]
-
-theorem getFin_eq_get {i : Nat} (hi : i < Size.size A.data) : A.getFin ⟨i, hi⟩ = A.get i := by
-  simp [get, hi]
-
-theorem getFin_eq_get' (i : Fin (Size.size A.data)) : A.getFin i = A.get i.val := by
-  simp [get]
-
-theorem get_push_lt {A : RangeArray α} {i : Nat} (hi : i < Size.size A.data) (v : α) :
-    (A.push v).get i = A.get i := by
-  simp [get, getFin, push, hi, Seq.get_snoc, lt_succ_of_lt hi]
-
-@[simp]
-theorem get_push_eq : (A.push v).get (Size.size A.data) = v := by
-  simp [get, getFin, push, Seq.get_snoc]
-
-theorem get_push_gt {A : RangeArray α} {i : Nat} (hi : i > Size.size A.data) (v : α) :
-    (A.push v).get i = default := by
-  replace hi := succ_le_of_lt hi
-  rw [succ_eq_add_one] at hi
-  have := (not_lt.mpr hi)
-  simp [get, push, Seq.size_snoc, this]
-
-theorem get_clear_lt {A : RangeArray α} {i : Nat} (hi : i < A.dsize) :
-    (A.clear).get i = A.get i := by
-  simp [clear, get, hi, usize]
-  split <;> rename _ => h_usize
-  · simp [getFin_eq_get, h_usize]
-  · have h_dsize : dsize A < LeanColls.size A.data := by omega
-    split <;> rename _ => hi'
-    · simp [LeanColls.size] at hi'
-      simp [getFin_eq_get, h_usize]
-      simp [get, hi, LeanColls.size, hi', getFin]
-      have := List.getElem_take A.data.data (lt_trans hi h_dsize) hi'.1
-      simp [Seq.get, getElem_eq_data_getElem, this]
-    · simp [LeanColls.size, hi] at hi'
-      have := lt_trans hi h_dsize
-      exact absurd this (not_lt_of_ge hi')
-
-theorem get_clear_ge {A : RangeArray α} {i : Nat} (hi : i ≥ A.dsize) :
-    (A.clear).get i = default := by
-  simp [clear, get, hi, usize]
-  split <;> rename _ => h_usize
-  · simp [getFin_eq_get, h_usize]
-    have : A.dsize ≥ LeanColls.size A.data := by omega
-    intro h_con
-    exact absurd (lt_of_lt_of_le h_con this) (not_lt_of_ge hi)
-  · simp [LeanColls.size, hi]
-
-theorem get_commit_lt {A : RangeArray α} {i : Nat} (hi : i < Size.size A.data) :
-    (A.commit).get i = A.get i := by
-  simp [get, getFin, commit, hi, usize]
-
-theorem get_commit_lt_usize {A : RangeArray α} {i : Nat} (hi : i < A.usize) :
-    (A.commit).get (A.dsize + i) = A.get (A.dsize + i) := by
-  simp [get, getFin, commit, hi, usize]
-
-/- theorem get_append_lt {A : RangeArray α} {i : Nat} (hi : i < A.dsize) (arr : Array α) :
-    (A.append arr).get i = A.get i := by -/
-
-/-
-theorem get_append_ge {A : RangeArray α} {i : Nat} (hi : i ≥ A.dsize) (arr : Array α) :
-    (A.append arr).get i = arr.get (i - A.dsize) := by -/
+/-! # oget and uget -/
 
 theorem indexFin_add_rsizeFin_le_size {A : RangeArray α}
       (i : Fin A.size) :
@@ -913,523 +395,50 @@ theorem indexFin_add_offset_lt_size {A : RangeArray α}
   have := indexFin_add_rsizeFin_le_size i
   apply lt_of_lt_of_le (by omega) this
 
-theorem index_add_offset_lt_size {A : RangeArray α} {i offset : Nat}
-      (hi : i < A.size) (ho : offset < A.rsize i) :
-    A.index i + offset < Size.size A.data := by
-  have := indexFin_add_offset_lt_size ⟨i, hi⟩ ⟨offset, by rw [rsizeFin_eq_rsize]; exact ho⟩
-  rw [indexFin_eq_index] at this
-  exact this
-
-/-! # oget and uget -/
-
 @[inline, always_inline]
 def ogetFin {A : RangeArray α} (i : Fin A.size) (offset : Fin (A.rsizeFin i)) : α :=
-  A.getFin ⟨A.indexFin i + offset.val,
-      indexFin_add_offset_lt_size i offset⟩
+  A.getFin ⟨A.indexFin i + offset.val, indexFin_add_offset_lt_size i offset⟩
 
 @[inline, always_inline]
-def oget (i offset : Nat) : α :=
+def oget [Inhabited α] (i offset : Nat) : α :=
   if hi : i < A.size then
     if ho : offset < A.rsizeFin ⟨i, hi⟩ then
       A.ogetFin ⟨i, hi⟩ ⟨offset, ho⟩
     else default
   else default
 
-theorem ogetFin_eq_oget {i offset : Nat} (hi : i < A.size) (ho : offset < A.rsizeFin ⟨i, hi⟩) :
-    A.ogetFin ⟨i, hi⟩ ⟨offset, ho⟩ = A.oget i offset := by
-  simp [oget, hi, ho]
-
-theorem ogetFin_eq_oget' (i : Fin A.size) (offset : Fin (A.rsizeFin i)) :
-    A.ogetFin i offset = A.oget i.val offset.val := by
-  simp [oget]
-
-theorem ogetFin_eq_getFin {i offset : Nat} (hi : i < A.size) (ho : offset < A.rsizeFin ⟨i, hi⟩) :
-    A.ogetFin ⟨i, hi⟩ ⟨offset, ho⟩ =
-      A.getFin ⟨A.indexFin ⟨i, hi⟩ + offset, indexFin_add_offset_lt_size ⟨_, hi⟩ ⟨_, ho⟩⟩ := by
-  simp [ogetFin]
-
 @[inline, always_inline]
 def ugetFin {A : RangeArray α} (i : Fin A.usize) : α :=
   A.getFin ⟨A.dsize + i.val, Nat.add_lt_of_lt_sub' i.isLt⟩
 
 @[inline, always_inline]
-def uget (i : Nat) : α :=
+def uget [Inhabited α] (i : Nat) : α :=
   if hi : i < A.usize then
     A.ugetFin ⟨i, hi⟩
   else default
 
-theorem ugetFin_eq_uget {i : Nat} (hi : i < A.usize) : A.ugetFin ⟨i, hi⟩ = A.uget i := by
-  simp [uget, hi]
-
-theorem ugetFin_eq_uget' (i : Fin A.usize) : A.ugetFin i = A.uget i.val := by
-  simp [uget]
-
-@[simp]
-theorem oget_push (A : RangeArray α) (i offset : Nat) (v : α) :
-    (A.push v).oget i offset = A.oget i offset := by
-  simp [oget, ogetFin]
-  split <;> try rfl
-  rename _ => hi
-  split <;> try rfl
-  rename _ => ho
-  rw [rsizeFin_eq_rsize] at ho
-  have h_add := indexFin_add_rsizeFin_le_size ⟨i, hi⟩
-  simp_rw [getFin_eq_get, indexFin_eq_index, rsizeFin_eq_rsize] at h_add ⊢
-  have : index A i + offset < index A i + rsize A i := by omega
-  have := lt_of_lt_of_le this h_add
-  simp [get_push_lt this v]
-
-theorem oget_commit_lt {A : RangeArray α} {i offset : Nat} (hi : i < A.size) (ho : offset < A.rsize i) :
-    (A.commit).oget i offset = A.oget i offset := by
-  simp [oget, ogetFin, hi, lt_succ_of_lt hi]
-  simp_rw [rsizeFin_eq_rsize, getFin_eq_get, indexFin_eq_index]
-  simp [ho, index_commit_lt hi]
-  apply get_commit_lt
-  exact index_add_offset_lt_size hi ho
-
-theorem oget_commit_eq {A : RangeArray α} {offset : Nat} (ho : offset < A.usize) :
-    (A.commit).oget A.size offset = A.uget offset := by
-  simp [oget, ogetFin, uget, ugetFin, ho]
-  simp_rw [indexFin_eq_index, getFin_eq_get]
-  simp
-  apply get_commit_lt
-  simp [usize] at ho
-  omega
-
-theorem oget_delete_ne (A : RangeArray α) {i j offset : Nat} (hij : i ≠ j) :
-    (A.delete i).oget j offset = A.oget j offset := by
-  simp [delete]
-  split <;> rename _ => hi <;> try rfl
-  simp [oget, ogetFin]
-  split <;> rename _ => hj <;> try rfl
-  simp_rw [rsizeFin_eq_rsize, deleteFin_eq_delete]
-  simp [rsize_delete_ne hij]
-  split <;> rename _ => ho <;> try rfl
-  simp [getFin, deleteFin, indexFin, Seq.get_set, hij]
-
-theorem uget_push_lt {A : RangeArray α} {i : Nat} (hi : i < A.usize) (v : α) :
-    (A.push v).uget i = A.uget i := by
-  simp [uget, ugetFin, hi, lt_succ_of_lt hi]
-  simp_rw [getFin_eq_get]
-  apply get_push_lt
-  simp [usize] at hi
-  omega
-
-@[simp]
-theorem uget_push_eq : (A.push v).uget A.usize = v := by
-  simp [uget, ugetFin]
-  rw [getFin_eq_get]
-  simp [usize]
-  rw [← Nat.add_sub_assoc A.h_size, Nat.add_comm, Nat.add_sub_cancel]
-  exact get_push_eq _ _
-
-@[simp]
-theorem uget_delete (A : RangeArray α) (i j : Nat) :
-    (A.delete j).uget i = A.uget i := by
-  simp [delete]
-  split <;> rfl
-
 /-! # models -/
 
+/--
+  A `RangeArray` models a 2D array of data, and an uncommitted list of data,
+  if it agrees with the data at all indexes, and if the two agree on
+  deleted indexes.
+
+  Note that for `h_agree` and `h_uncommitted`, we use `.oget` and `.uget`
+  rather than `.ogetFin` and `.ugetFin` because Lean struggles to close
+  proof goals with slightly "wrong" dependent inequality proofs.
+-/
 structure models (R : RangeArray α) (Ls : List (Option (List α))) (L : List α) : Prop where
   (h_size₁ : R.size = Size.size Ls)
   (h_size₂ : R.usize = Size.size L)
   (h_some : ∀ {i : Nat} (hi : i < Size.size Ls),
     (R.isDeleted i = false) ↔ (∃ (C : List α), Seq.get Ls ⟨i, hi⟩ = some C))
   (h_sizes : ∀ {i : Nat} (hi : i < Size.size Ls) {sL : List α},
-    Seq.get Ls ⟨i, hi⟩ = some sL → R.rsize i = Size.size sL)
-  (h_agree : ∀ {i : Nat} (hi : i < Size.size Ls) {sL : List α},
-      Seq.get Ls ⟨i, hi⟩ = some sL →
+    Seq.get Ls ⟨i, hi⟩ = some sL → R.rsizeFin ⟨i, h_size₁ ▸ hi⟩ = Size.size sL)
+  (h_agree : ∀ {i : Nat} (hi : i < Size.size Ls) {sL : List α} (hsL : Seq.get Ls ⟨i, hi⟩ = some sL),
         (∀ {j : Nat} (hj : j < (Size.size sL)),
-          R.oget i j = Seq.get sL ⟨j, hj⟩))
+          R.ogetFin ⟨i, h_size₁ ▸ hi⟩ ⟨j, (h_sizes hi hsL) ▸ hj⟩ = Seq.get sL ⟨j, hj⟩))
   (h_uncommitted : ∀ {i : Nat} (hi : i < Size.size L),
-      R.uget i = Seq.get L ⟨i, hi⟩)
-
-variable {R : RangeArray α} {Ls : List (Option (List α))} {L : List α} (h_models : models R Ls L)
-
-theorem get_eq_some_of_models_of_not_deleted {i : Nat} :
-    R.isDeleted i = false → ∃ (hi : i < Size.size Ls) (sL : _), Seq.get Ls ⟨i, hi⟩ = some sL := by
-  intro h_del
-  by_cases hi : i < Size.size Ls
-  · have := h_models.h_some hi
-    simp [h_del] at this
-    use hi
-  · rw [← h_models.h_size₁] at hi
-    rw [isDeleted_true_of_ge (not_lt.mp hi)] at h_del
-    contradiction
-
-@[simp]
-theorem models_empty (size : Nat) : models (empty size) ([] : List (Option (List α))) [] := by
-  constructor <;> simp
-
-theorem models_push : ∀ (v : α), models (R.push v) Ls (Seq.snoc L v) := by
-  intro v
-  constructor
-  · simp [h_models.h_size₁]
-  · simp [h_models.h_size₂]
-  · refine h_models.h_some
-  · refine h_models.h_sizes
-  · intro i hi sL hsL j hj
-    simp [h_models.h_agree hi hsL hj]
-  · intro i hi
-    have hi₁ := hi
-    rw [Seq.size_snoc, ← h_models.h_size₂] at hi₁
-    rcases eq_or_lt_of_le (le_of_lt_succ hi₁) with (hi' | hi')
-    · conv => lhs; simp [hi']
-      rw [h_models.h_size₂] at hi'
-      simp [Seq.get_snoc, hi']
-    · conv => lhs; simp [uget_push_lt hi']
-      rw [Seq.get_snoc]
-      rw [h_models.h_size₂] at hi'
-      split <;> rename _ => hi₂
-      · exact h_models.h_uncommitted hi'
-      · simp at hi₂ hi
-        have := le_antisymm hi₂ (le_of_lt_succ hi)
-        rw [this] at hi'
-        exact absurd hi' (not_lt.mpr (le_refl _))
-
-theorem models_commit : models (R.commit) (Seq.snoc Ls (some L)) [] := by
-  constructor
-  · simp [h_models.h_size₁]
-  · simp [h_models.h_size₂]
-  · intro i hi
-    have hi₁ := hi
-    simp at hi₁
-    simp [Seq.get_snoc, -eq_iff_iff]
-    split <;> rename _ => hi₂
-    · rw [← h_models.h_size₁] at hi₂
-      conv => lhs; simp [isDeleted_commit_lt hi₂]
-      rw [h_models.h_size₁] at hi₂
-      exact h_models.h_some hi₂
-    · simp only [not_lt] at hi₂
-      have := le_antisymm (le_of_lt_succ hi₁) hi₂
-      rw [← h_models.h_size₁] at this
-      simp [this]
-  · intro i hi sL hsL
-    simp at hi
-    rcases eq_or_lt_of_le (le_of_lt_succ hi) with (rfl | hi₂)
-    · conv => lhs; rw [← h_models.h_size₁]
-      simp [h_models.h_size₂]
-      simp [Seq.get_snoc] at hsL
-      subst hsL
-      rfl
-    · rw [← h_models.h_size₁] at hi₂
-      rw [rsize_commit_lt hi₂]
-      rw [h_models.h_size₁] at hi₂
-      simp [Seq.get_snoc, hi₂] at hsL
-      exact h_models.h_sizes hi₂ hsL
-  · intro i hi sL hsL j hj
-    have hi₁ := hi
-    simp at hi₁
-    rcases eq_or_lt_of_le (le_of_lt_succ hi₁) with (hi₂ | hi₂)
-    · simp [hi₂] at hsL
-      subst hsL
-      rw [← h_models.h_size₁] at hi₂
-      rw [hi₂, oget_commit_eq ((h_models.h_size₂).symm ▸ hj)]
-      exact h_models.h_uncommitted hj
-    · simp [Seq.get_snoc, hi₂] at hsL
-      rw [← h_models.h_sizes hi₂ hsL] at hj
-      rw [← h_models.h_size₁] at hi₂
-      rw [oget_commit_lt hi₂ hj]
-      rw [h_models.h_size₁] at hi₂
-      rw [h_models.h_sizes hi₂ hsL] at hj
-      exact h_models.h_agree hi₂ hsL hj
-  · simp
-
-theorem models_delete : ∀ {i : Nat} (hi : i < Size.size Ls),
-    models (R.delete i) (Seq.set Ls ⟨i, hi⟩ none) L := by
-  intro i hi
-  constructor
-  · simp [h_models.h_size₁]
-  · simp [h_models.h_size₂]
-  · intro j hj
-    by_cases hij : i = j
-    · simp [hij]
-    · rw [isDeleted_delete_ne R hij]
-      simp [Seq.get_set, hij, -eq_iff_iff]
-      simp at hj
-      exact h_models.h_some hj
-  · intro j hj sL hsL
-    by_cases hij : i = j
-    · simp [Seq.get_set, hij] at hsL
-    · simp [Seq.get_set, hij] at hsL
-      simp at hj
-      rw [rsize_delete_ne hij]
-      exact h_models.h_sizes hj hsL
-  · intro j hj sL hsL k hk
-    by_cases hij : i = j
-    <;> simp [Seq.get_set, hij] at hsL
-    simp at hj
-    have := h_models.h_some hj
-    simp [hsL] at this
-    rw [oget_delete_ne R hij]
-    exact h_models.h_agree hj hsL hk
-  · intro j hj
-    simp [uget_delete]
-    exact h_models.h_uncommitted hj
-
-theorem eq_nil_of_models_of_usize_zero : R.usize = 0 → L = [] := by
-  intro h_usize
-  rw [h_models.h_size₂] at h_usize
-  simp [LeanColls.size] at h_usize
-  -- There's probably a one-line proof here
-  cases L with
-  | nil => rfl
-  | cons _ _ => simp at h_usize
-
-/-! # drop and take -/
-
-/-def drop (A : RangeArray α) : RangeArray α :=
-
-theorem models_cons {R : RangeArray α} {x : α} {xs : List α} {Ls : Option (List α)} {L : List α}
-  (h_models : R)
-
-#exit -/
-
--- CC: Which direction does this theorem need to be in?
-/- theorem exists_model (A : RangeArray α) :
-    ∃ (Ls : List (Option (List α))) (L : List α), models A Ls L := by -/
-
-/- theorem exists_model' (Ls : List (Option (List α))) (L : List α) :
-    ∃ (A : RangeArray α), models A Ls L := by -/
-
-/-! # fold -/
-
-@[inline, always_inline, specialize]
-def foldlM_index {β : Type v} {m : Type v → Type w} [Monad m] (f : β → α → m β)
-    (init : β) (A : RangeArray α) (i : Nat) : m β :=
-  if isDeleted A i = false then
-    A.data.foldlM f init (A.index i) (A.index i + A.rsize i)
-  else return init
-
-@[inline, always_inline, specialize]
-def foldl_index {β : Type v} (f : β → α → β)
-    (init : β) (A : RangeArray α) (i : Nat) : β :=
-  if isDeleted A i = false then
-    A.data.foldl f init (A.index i) (A.index i + A.rsize i)
-  else init
-
-@[inline, always_inline, specialize]
-def foldlM_indexHyps {β : Type v} {m : Type v → Type w} [Monad m] (f : β → α → m β)
-    (init : β) (A : RangeArray α) (i : Fin A.size) : m β :=
-  if isDeleted A i = false then
-    A.data.foldlM f init (A.indexFin i) (A.indexFin i + A.rsizeFin i)
-  else return init
-
-@[inline, always_inline, specialize]
-def foldl_indexHyps {β : Type v} (f : β → α → β)
-    (init : β) (A : RangeArray α) (i : Fin A.size) : β :=
-  if isDeleted A i = false then
-    A.data.foldl f init (A.indexFin i) (A.indexFin i + A.rsizeFin i)
-  else init
-
-@[inline, always_inline, specialize]
-def ufoldlM {β : Type v} {m : Type v → Type w} [Monad m] (f : β → α → m β)
-    (init : β) (A : RangeArray α) : m β :=
-  A.data.foldlM f init A.dsize (A.dsize + A.usize)
-
-@[inline, always_inline, specialize]
-def ufoldl {β : Type v} (f : β → α → β)
-    (init : β) (A : RangeArray α) : β :=
-  A.data.foldl f init A.dsize (A.dsize + A.usize)
-
-def foldlM_index_looped {β : Type v} {m : Type v → Type w} [Monad m] (f : β → α → m β)
-    (init : β) (A : RangeArray α) (i : Nat) : m β :=
-  if isDeleted A i = false then
-    let rec loop (j : Nat) (b : β) : m β := do
-      if j < A.rsize i then
-        loop (j + 1) (← f b (A.oget i j))
-      else return b
-    termination_by A.rsize i - j
-    loop 0 init
-  else return init
-
-/-
-theorem unitProp.go.cons_aux (τ : PPA) (l : ILit) {ls : List ILit} {i j : Nat} :
-    j = ls.length - i → unitProp.go τ { data := l :: ls } (i + 1) = unitProp.go τ { data := ls } i := by
-
-    /-- Invariants -/
-
-  h_size : dataSize ≤ Size.size data
-  h_dataSize_empty : Size.size indexes = 0 → dataSize = 0
-
-  -- No index exceeds `dataSize`
-  h_indexes : ∀ {i : Nat} (hi : i < Size.size indexes),
-    RangeArray.getIndexFromMarkedIndex (Seq.get indexes ⟨i, hi⟩) ≤ dataSize
-
-  -- The indexes are monotonically increasing in (unmarked) value
-  h_indexes_inc : ∀ {i j : Nat} (hij : i ≤ j) (hj : j < Size.size indexes),
--/
-
---theorem foldlM_index_looped.loop.cons_aux
-
-/-theorem foldlM_index_looped_eq_foldlM_index {β : Type v} {m : Type v → Type w} [Monad m]
-    (f : β → α → m β) (init : β) (A : RangeArray α) (i : Nat) :
-      A.foldlM_index_looped f init i = A.foldlM_index f init i := by
-  have ⟨data, indexes, dataSize, _, h_size, h_dataSize_empty, h_indexes, h_indexes_inc⟩ := A
-  have ⟨data⟩ := data
-  have ⟨indexes⟩ := indexes
-  simp [foldlM_index_looped, foldlM_index]
-  induction data with
-  | nil =>
-    simp [foldlM, foldlM_index]
-  | cons x xs ih =>
-    simp [foldlM, foldlM_index]
-    rw [ih]
-    simp [foldlM_index_looped]
-
-#exit -/
-
-/-
-theorem unitProp.go.cons_aux (τ : PPA) (l : ILit) {ls : List ILit} {i j : Nat} :
-    j = ls.length - i → unitProp.go τ { data := l :: ls } (i + 1) = unitProp.go τ { data := ls } i := by
-  intro hj
-  ext unit?
-  induction j generalizing τ unit? i with
-  | zero =>
--/
-
-#check LeanColls.Seq
-#check Option.bind
-theorem foldlM_index_eq_foldlM {i : Nat} {hi : i < Size.size Ls}
-    {sL : List α} (hsL : Seq.get Ls ⟨i, hi⟩ = some sL)
-    {β : Type v} {m : Type v → Type w} [Monad m] (f : β → α → m β) (init : β) :
-    R.foldlM_index f init i = sL.foldlM f init := by
-  have ⟨data, indexes, dataSize, _, h_size, h_dataSize_empty, h_indexes, h_indexes_inc⟩ := A
-  have ⟨data⟩ := data
-  have ⟨indexes⟩ := indexes
-  rw [foldlM_index]
-  have := h_models.h_some hi
-  simp [hsL] at this
-  simp [this]
-  sorry
-  /-induction sL generalizing Ls with
-  | nil =>
-    have := h_models.h_sizes hi hsL
-    simp at this
-    simp [this]
-  | cons x xs ih =>
-    stop
-    done -/
-  done
-
-#exit
-
-
-@[simp]
-theorem foldlM_index_empty {β : Type v} {m : Type v → Type w} [Monad m]
-    (f : β → α → m β) (init : β) (i : Nat) :
-      (empty : RangeArray α).foldlM_index f init i = return init := by
-  simp [foldlM_index, empty]
-
-@[simp]
-theorem foldl_index_empty {β : Type v} (f : β → α → β) (init : β) (i : Nat) :
-      (empty : RangeArray α).foldl_index f init i = init := by
-  simp [foldl_index, empty]
-
-@[simp]
-theorem foldlM_index_add {β : Type v} {m : Type v → Type w} [Monad m]
-    (f : β → α → m β) (init : β) (arr : Array α) (i : Nat) :
-      (A.add arr).foldlM_index f init i =
-        if i = A.size then arr.foldlM f init
-        else A.foldlM_index f init i := by
-  simp [foldlM_index, add, foldlM]
-  sorry
-
-@[simp]
-theorem foldl_index_add {β : Type v} (f : β → α → β) (init : β) (arr : Array α) (i : Nat) :
-      (A.add arr).foldl_index f init i =
-        if i = A.size then arr.foldl f init
-        else A.foldl_index f init i := by
-  simp [foldl_index, empty, foldlM_index_empty]
-  sorry
-
-theorem foldlM_index_trivial {β : Type v} {m : Type v → Type w} [Monad m]
-    {A : RangeArray α} {i : Nat} : (A.rsize i) = 0 →
-      ∀ (f : β → α → m β) init, A.foldlM_index f init i = return init := by
-  sorry
-
-theorem foldl_index_trivial {β : Type v} {A : RangeArray α} {i : Nat} :
-    (A.rsize i) = 0 → ∀ (f : β → α → β) init, A.foldl_index f init i = init := by
-  intro hr
-  simp [foldl_index, Array.foldl]
-  sorry
-
-@[inline]
-def foldlM {β : Type v} {m : Type v → Type w} [Monad m]
-    (g : β → α → m β) (f : β → β → m β)
-    (initg initf : β) (A : RangeArray α)
-    (start : Nat := 0) (stop : Nat := A.size) : m β :=
-  let minStop := min stop A.size
-  let rec loop (i : Nat) (b : β) : m β := do
-    if h : i < minStop then
-      loop (i + 1) (
-        if !A.isDeleted i then
-          ← f b (← A.foldlM_index g initg i)
-        else b)
-    else return b
-  termination_by minStop - i
-  loop start initf
-
-@[inline]
-def foldlM_over_indexes {β : Type v} {m : Type v → Type w} [Monad m]
-    (f : β → Nat → m β) (init : β) (A : RangeArray α)
-    (start : Nat := 0) (stop : Nat := A.size) : m β :=
-  let minStop := min stop A.size
-  let rec loop (i : Nat) (b : β) : m β := do
-    if h : i < minStop then
-      loop (i + 1) (
-        if !A.isDeleted i then
-          ← f b i
-        else b)
-    else return b
-  termination_by minStop - i
-  loop start init
-
-@[inline]
-def foldl_over_indexes {β : Type v}
-    (f : β → Nat → β) (init : β) (A : RangeArray α)
-    (start : Nat := 0) (stop : Nat := A.size) : β :=
-  Id.run <| A.foldlM_over_indexes f init start stop
-
-@[inline]
-def foldl {β : Type v} (g : β → α → β) (f : β → β → β)
-    (initg initf : β) (A : RangeArray α) (start : Nat := 0) (stop : Nat := A.size) :=
-  Id.run <| A.foldlM g f initg initf start stop
---Fin.foldRange (fun i b => f_outer b (A.foldl_index f_inner init_inner i)) init_outer start stop
-
-@[simp]
-theorem foldlM_empty {β : Type v} {m : Type v → Type w} [Monad m]
-    (g : β → α → m β) (f : β → β → m β) (initg initf : β) (start stop : Nat) :
-      (empty : RangeArray α).foldlM g f initg initf start stop = return initf := by
-  stop
-  simp [RangeArray.foldlM]
-  simp [foldlM, empty]
-  rintro rfl
-  exact Array.foldlM_empty _ _ _ _
-
-@[simp]
-theorem foldl_empty {β : Type v} (g : β → α → β) (f : β → β → β)
-    (initg initf : β) (start stop : Nat) :
-      (empty : RangeArray α).foldl g f initg initf start stop = initf := by
-  simp [foldl, Id.run]
-
-theorem foldlM_add {β : Type v} {m : Type v → Type w} [Monad m]
-    (g : β → α → m β) (f : β → β → m β) (initg initf : β)
-    (A : RangeArray α) (arr : Array α) :
-      (A.add arr).foldlM g f initg initf = do
-        { f (← A.foldlM g f initg initf) (← arr.foldlM g initg) } := by
-  stop
-  done
-
-theorem foldl_add {β : Type v} (g : β → α → β) (f : β → β → β)
-    (initg initf : β) (A : RangeArray α) (arr : Array α) :
-      (A.add arr).foldl g f initg initf = f (A.foldl g f initg initf) (arr.foldl g initg) := by
-  --simp [foldl, foldlM_add]
-  --intro hi f init
-  simp [Array.foldl, Id.run]
-  --exact foldlM_add (m := Id) g f initg initf _ _
-  sorry
-  done
+      R.ugetFin ⟨i, h_size₂ ▸ hi⟩ = Seq.get L ⟨i, hi⟩)
 
 end RangeArray
