Experiments/ProofChecking/Parsing/BStreamParser.lean
@@ -1,0 +1,119 @@
+/-
+
+A CNF and SR parser from buffered streams (`BStream`).
+
+Author: Cayden Codel
+Carnegie Mellon University
+
+-/
+
+import Experiments.ProofChecking.BStream
+import Experiments.ProofChecking.UInt
+import Experiments.ProofChecking.Parsing.Defs
+
+import Lean.Exception
+import LeanSAT.Solver.Dimacs
+import Experiments.ProofChecking.RangeArray
+
+open Batteries
+open LeanSAT.Solver.Dimacs
+open LeanSAT LeanSAT.Model ILit Except
+open LeanColls
+
+namespace BStreamParser
+
+open IO.FS BStream Parsing
+
+variable {CNF : Type _} [Formula CNF] [Inhabited CNF]
+
+@[inline, specialize]
+partial def parseClause (maxVar : Nat) (F : CNF) : BStreamM CNF := do
+  -- Just keep parsing literals until 0 is encountered
+  let lit ← readInt!
+  if h_lit : lit = 0 then
+    return Formula.commitClause F
+  else
+    if lit.natAbs > maxVar then
+      panic! s!"Error: Literal {lit} exceeds maximum variable {maxVar}"
+    else
+      let F := Formula.addLiteral F ⟨lit, h_lit⟩
+      parseClause maxVar F
+
+@[inline, specialize]
+partial def parseFormula : BStreamM (CNF × Nat) := do
+  let F := Formula.empty
+  --let problemLine ←
+  let foundProblemLine ← scanMatch "p cnf"
+  if !foundProblemLine then
+    panic! "Error: Expected problem line"
+
+  -- Get the number of vars and number of clauses
+  let nVars ← readNat!
+  let nClauses ← readNat!
+
+  let rec loop (i : Nat) (F : CNF) : BStreamM CNF := do
+    if i ≥ nClauses then
+      return F
+    else
+      let F ← parseClause nVars F
+      loop (i + 1) F
+
+  let F ← loop 0 F
+
+  if Formula.size F ≠ nClauses then
+    panic! "Error: Expected {nClauses} clauses, but got {Formula.size F}"
+
+  return (F, nVars)
+
+partial def parseLSRDeletionline : BStreamM SRDeletionLine := do
+  -- Read nats until 0 is encountered
+  let rec loop (acc : Array Nat) := do
+    let clauseId ← readNat!
+    if clauseId = 0 then
+      return { clauses := acc }
+    else
+      loop (acc.push (clauseId - 1))
+  loop #[]
+
+/-
+instance : Inhabited (Nat × CNF × (SRAdditionLine ⊕ SRDeletionLine)) := ⟨0, Formula.empty, Sum.inl SRAdditionLine.new⟩
+instance : Inhabited (BStreamM (Nat × CNF × (SRAdditionLine ⊕ SRDeletionLine))) := ⟨fun σ => return (⟨0, Formula.empty, Sum.inl SRAdditionLine.new⟩, σ)⟩
+-/
+
+@[specialize]
+partial def parseLSRLine (F : CNF) : BStreamM (Nat × CNF × (SRAdditionLine ⊕ SRDeletionLine)) := do
+  -- Keep parsing ints until a 0 is found
+  let lineId ← readNat!
+  ws
+
+  -- Check whether a 'd' char indicates a deletion line
+  let delCh? ← getc!
+  if delCh? = 'd'.toUInt8 then
+    let delLine ← parseLSRDeletionline
+    return (lineId, F, Sum.inr delLine)
+  else
+    -- Addition line!
+    ungetc delCh?
+    let F := Formula.commitClauseUntil F (lineId - 1)
+
+    -- Parse the clause (lits until a repeat of the pivot, or 0)
+    let pivot ← readInt!
+    let line := SRAdditionLine.new
+    let state :=
+      if h : pivot = 0 then
+        ParsingState.mk .upHints none F line
+      else
+        ParsingState.mk .clause (some ⟨pivot, h⟩) (Formula.addLiteral F ⟨pivot, h⟩) line
+
+    -- Process the line until we get .lineDone
+    let rec loop (state : ParsingState CNF) := do
+      let atom ← readInt!
+      let ⟨mode, pivot, F, line⟩ := processSRAtom atom state
+      match mode with
+      | .lineDone => return (lineId, F, Sum.inl line)
+      | .err s => panic! s!"LSR parsing error: {s}"
+      | _ => loop ⟨mode, pivot, F, line⟩
+
+    loop state
+
+end BStreamParser
