Experiments/ProofChecking/Parsing/BStreamParserExe.lean
@@ -1,0 +1,49 @@
+import Experiments.ProofChecking.BStream
+import Experiments.ProofChecking.RangeArray
+import Experiments.ProofChecking.Parsing.Defs
+import Experiments.ProofChecking.Parsing.BStreamParser
+
+open LeanSAT LeanSAT.Model ILit Except IO.FS
+
+def printUsage : IO Unit := do
+  IO.println "Usage: ./BStreamParser <file_path> [cnf | lsr | clsr]"
+
+def echoCNF (filePath : String) : IO Unit := do
+  let bs ← BStream.ofFilePath filePath
+  let ((F, nVars), _) ← @BStreamParser.parseFormula (RangeArray ILit) _ _ bs
+
+  IO.println s!"p cnf {nVars} {F.size}"
+  Parsing.echoRangeArrayCNF F
+
+@[specialize]
+partial def echoLSR (filePath : String) (F : RangeArray ILit) : IO Unit := do
+  let bs ← BStream.ofFilePath filePath
+  let rec loop (F : RangeArray ILit) : BStreamM (RangeArray ILit):= do
+    BStream.ws
+    let ch ← BStream.getc
+    if ch = EOF then
+      return F
+    else
+      BStream.ungetc ch.toUInt8
+      let (lineId, F, line) ← BStreamParser.parseLSRLine F
+      --Parsing.echoRangeArrayLSRLine F lineId line
+      let F := F.commit
+      loop F
+  let t₁ ← IO.monoMsNow
+  let (F, _) ← loop F bs
+  let t₂ ← IO.monoMsNow
+  IO.println s!"Number of addition lines parsed: {F.size}"
+  IO.println s!"Time taken: {t₂ - t₁} ms"
+
+def echoLSRBinary (filePath : String) : IO Unit := do
+  IO.println "Not implemented"
+
+def main : List String → IO Unit
+  | [] => printUsage
+  | filePath :: args => do
+    match args with
+    | [] => echoLSR filePath (RangeArray.empty)
+    | ["cnf"] => echoCNF filePath
+    | ["lsr"] => echoLSR filePath (RangeArray.empty)
+    --| ["clsr"] => echoLSRBinary filePath
+    | _ => printUsage
